specs/Spec.Kraft.fsti
@@ -2,6 +2,7 @@ module Spec.Kraft
 
 module UInt = FStar.UInt
 module Math = FStar.Math.Lemmas
+module MathLib = FStar.Math.Lib
 
 open FStar.Mul
 open FStar.Seq
@@ -9,36 +10,282 @@ open Lib.Seq
 open Lib.Rational
 
 type tree = 
-  | Node: left: tree -> right: tree -> tree
-  | Leaf: symbol: nat -> tree
+  | Node: left: tree -> freq: pos -> right: tree -> tree
+  | Leaf: symbol: nat -> freq: pos -> tree
 
 type non_leaf = t: tree{Leaf? t == false}
 
 unfold let left (t: non_leaf) =
   match t with
-  | Node l _ -> l
+  | Node l _ _ -> l
 
 unfold let right (t: non_leaf) =
   match t with
-  | Node _ r -> r
+  | Node _ _ r -> r
+
+unfold let freq (t: tree) =
+  match t with
+  | Node _ f _ -> f
+  | Leaf _ f -> f
+
+let rec symbols (t: tree) =
+  match t with
+  | Node l _ r -> symbols l @| symbols r
+  | Leaf s _ -> create 1 s
+
+type tree_symbol (t: tree) = s: nat{
+  Seq.mem s (symbols t)
+}
+
+let rec code_length (t: tree) (s: tree_symbol t) =
+  match t with
+  | Node l _ r ->
+    let ls = symbols l in
+    let rs = symbols r in
+    lemma_mem_append ls rs;
+    1 + (if Seq.mem s ls then code_length l s else code_length r s)
+  | _ -> 0
+
+let rec code_freq (t: tree) (s: tree_symbol t) =
+  match t with
+  | Node l _ r ->
+    let ls = symbols l in
+    let rs = symbols r in
+    lemma_mem_append ls rs;
+    if Seq.mem s ls then code_freq l s else code_freq r s
+  | Leaf _ f -> f
 
 let rec height (t: tree): Tot nat =
   match t with
-  | Node l r ->
+  | Node l _ r ->
     let lh = height l in let rh = height r in
     1 + (if lh > rh then lh else rh)
   | _ -> 0
 
+type tree_height (t: tree) = h: nat{
+  h <= height t
+}
+
+private let rec freq_pred (t: tree): Tot Type0 =
+  match t with
+  | Node l f r -> f == freq l + freq r /\ freq_pred l /\ freq_pred r
+  | _ -> True
+
+/// Definition of well-formed trees. Their root frequencies should be the sum of
+/// the children's frequency, and their symbol list should not have duplicated
+/// symbols.
+type wf_tree = t: tree{
+  no_dup (symbols t) /\ freq_pred t
+}
+
+let rec avg_len (t: tree): Tot nat =
+  match t with
+  | Node l f r -> f + avg_len l + avg_len r
+  | Leaf _ _ -> 0
+
+let optimal_tree = t: wf_tree{
+  forall (t': wf_tree{permutation nat (symbols t) (symbols t')}).
+    avg_len t <= avg_len t'
+}
+
+unfold let merge (l r: tree) = Node l (freq l + freq r) r
+
+unfold let subst_pre_cond (t: wf_tree) (s: tree_symbol t) (l' r': (nat & pos)): Tot Type0 =
+  let (sl, fl) = l' in
+  let (sr, fr) = r' in
+  sl <> sr /\ sl <> s /\ sr <> s /\
+  fl + fr == code_freq t s /\
+  mem sl (symbols t) == false /\
+  mem sr (symbols t) == false
+
+let rec subst (t: wf_tree) (s: tree_symbol t) (l' r': (nat & pos)): Pure tree
+  (requires subst_pre_cond t s l' r')
+  (ensures fun _ -> True) =
+ let (sl, fl) = l' in
+ let (sr, fr) = r' in
+  match t with
+  | Node l f r ->
+    lemma_append_count (symbols l) (symbols r);
+    if mem s (symbols l) then
+      Node (subst l s l' r') f r
+    else
+      Node l f (subst r s l' r')
+  | Leaf _ f ->
+    Node (Leaf sl fl) f (Leaf sr fr)
+
+let lemma_merge_subst
+  (l r: wf_tree) (s: tree_symbol (merge l r)) (l' r': (nat & pos)): Lemma
+  (requires (
+    let (sl, fl) = l' in
+    let (sr, fr) = r' in
+    disjoint (symbols l) (symbols r) /\
+    subst_pre_cond (merge l r) s l' r'))
+  (ensures (
+    let (sl, fl) = l' in
+    let (sr, fr) = r' in
+    lemma_append_count (symbols l) (symbols r);
+    (mem s (symbols l) ==> merge (subst l s l' r') r == subst (merge l r) s l' r') /\
+    (mem s (symbols r) ==> merge l (subst r s l' r') == subst (merge l r) s l' r'))) =
+  lemma_append_count (symbols l) (symbols r)
+
+#push-options "--z3rlimit 64 --fuel 0 --ifuel 0"
+[@"opaque_to_smt"]
+let rec min_freq_2 (f: seq wf_tree{length f >= 2}): Tot (res: (nat & nat){
+  let (i1, i2) = res in
+  i1 < length f /\ i2 < length f /\ i1 <> i2 /\
+  (forall i. freq f.[i1] <= freq f.[i]) /\
+  (forall i. i <> i1 ==> freq f.[i2] <= freq f.[i])
+}) (decreases length f) =
+  match length f with
+  | 2 ->
+    let f1 = freq f.[0] in
+    let f2 = freq f.[1] in
+    if f1 <= f2 then (0, 1) else (1, 0)
+  | _ ->
+    assert(forall i. i > 0 ==> f.[i] == (tail f).[i - 1]);
+    let (i1, i2) = min_freq_2 (tail f) in
+    let f0 = freq f.[0] in
+    if f0 < freq f.[i1 + 1] then
+      (0, i1 + 1)
+    else if f0 < freq f.[i2 + 1] then
+      (i1 + 1, 0)
+    else
+      (i1 + 1, i2 + 1)
+#pop-options
+
+let rec forest_symbols (f: seq wf_tree): Tot (seq nat) (decreases length f) =
+  match length f with
+  | 0 -> empty #nat
+  | _ -> symbols f.[0] @| forest_symbols (tail f)
+
+/// Definition of well-formed forest. Their symbol list should not have duplications.
+type wf_forest = f: seq wf_tree{
+  length f > 0 /\ no_dup (forest_symbols f)
+}
+
+let rec forest_avg_len (f: seq wf_tree{length f > 0}): Tot nat (decreases length f) =
+  match length f with
+  | 1 -> avg_len f.[0]
+  | _ -> avg_len f.[0] + forest_avg_len (tail f)
+
+let rec forest_symbols_begin (f: seq wf_tree{length f > 0}) (i: nat{i < length f}):
+  Tot nat (decreases i) =
+  match i with
+  | 0 -> 0
+  | _ -> length (symbols f.[0]) + forest_symbols_begin (tail f) (i - 1)
+
+let rec lemma_forest_symbols_begin (f: seq wf_tree{length f > 0}): Lemma
+  (ensures
+    forest_symbols_begin f (length f - 1) + length (symbols (last f)) ==
+    length (forest_symbols f))
+  (decreases length f) =
+  match length f with
+  | 1 -> ()
+  | _ -> lemma_forest_symbols_begin (tail f)
+
+#push-options "--z3refresh --fuel 1 --ifuel 1"
+let rec lemma_forest_symbols_index (f: seq wf_tree{length f > 0}) (i: nat{i < length f}): Lemma
+  (ensures (
+    let j = forest_symbols_begin f i in
+    let l = j + length (symbols f.[i]) in
+    l <= length (forest_symbols f) /\
+    slice (forest_symbols f) j l == symbols f.[i]))
+  (decreases i) =
+  match i with
+  | 0 ->
+    assert(equal (symbols f.[0]) (slice (forest_symbols f) 0 (length (symbols f.[0]))))
+  | _ ->
+    lemma_forest_symbols_index (tail f) (i - 1);
+    let j = forest_symbols_begin f i in
+    let l = j + length (symbols f.[i]) in
+    let o = length (symbols f.[0]) in
+    assert(equal
+      (slice (forest_symbols (tail f)) (j - o) (l - o))
+      (slice (slice (forest_symbols f) o (length (forest_symbols f))) (j - o) (l - o)))
+#pop-options
+
+let rec lemma_forest_symbols_unsnoc_1 (f: wf_forest {length f > 0}): Lemma
+  (ensures forest_symbols (unsnoc f) @| symbols (last f) == forest_symbols f)
+  (decreases length f) =
+  match length f with
+  | 1 -> assert(equal (forest_symbols (unsnoc f) @| symbols (last f)) (forest_symbols f))
+  | _ ->
+    lemma_forest_symbols_unsnoc_1 (tail f);
+    append_assoc (symbols f.[0]) (forest_symbols (unsnoc (tail f))) (symbols (last f))
+
+let rec lemma_forest_symbols_unsnoc_2 (f: wf_forest {length f > 0}): Lemma
+  (ensures no_dup (forest_symbols (unsnoc f)))
+  (decreases length f) =
+  match length f with
+  | 1 -> ()
+  | _ ->
+    lemma_forest_symbols_unsnoc_1 f;
+    lemma_forest_symbols_unsnoc_2 (tail f)
+
+#push-options "--z3refresh --z3rlimit 1024 --fuel 2 --ifuel 2"
+let rec lemma_wf_forest_symbols_disjoint (f: wf_forest{length f >= 2}) (i j: nat): Lemma
+  (requires i < j /\ j < length f)
+  (ensures 
+    no_dup (symbols f.[i]) /\
+    no_dup (symbols f.[j]) /\
+    disjoint (symbols f.[i]) (symbols f.[j]))
+  (decreases length f) =
+  let fs = forest_symbols f in
+  let fsbj = forest_symbols_begin f j in
+  let l0 = length (symbols f.[0]) in
+  let l1 = length (symbols f.[1]) in
+  lemma_forest_symbols_index f i;
+  lemma_forest_symbols_index f j;
+  if i = 0 then
+    if j = length f - 1 then begin
+      no_dup_slice fs l0 fsbj;
+      lemma_forest_symbols_begin f
+    end else if j = 1 then begin
+      no_dup_slice fs l0 (fsbj + l1);
+      lemma_forest_symbols_begin f
+    end else begin
+      lemma_forest_symbols_unsnoc_2 f;
+      lemma_wf_forest_symbols_disjoint (unsnoc f) i j
+    end
+  else
+    lemma_wf_forest_symbols_disjoint (tail f) (i - 1) (j - 1)
+#pop-options
+
+#push-options "--z3refresh --z3rlimit 1024 --fuel 2 --ifuel 2"
+let forest_reduce (f: wf_forest{length f >= 2}): Tot (f': wf_forest{
+  length f' == length f - 1
+}) =
+  let (i0, i1) = min_freq_2 f in
+  if i0 < i1 then
+    lemma_wf_forest_symbols_disjoint f i0 i1
+  else
+    lemma_wf_forest_symbols_disjoint f i1 i0;
+  match length f with
+  | 2 ->
+    admit();
+    let res = create 1 (merge f.[i0] f.[i1]) in
+    let t = merge f.[i0] f.[i1] in
+    create 1 (merge f.[i0] f.[i1])
+  | _ ->
+    let t' = merge f.[i0] f.[i1] in
+    let f' = remove f i0 in
+    let f'' = remove f' (if i0 < i1 then i1 - 1 else i1) in
+    assert(no_dup (symbols t'));
+    assert(permutation nat (symbols t') (symbols f.[i0] @| symbols f.[i1]));
+    admit();
+    create 1 t' @| f''
+#pop-options
+
 let rec leaf_count (t: tree): Tot pos = 
   match t with
-  | Node l r -> leaf_count l + leaf_count r
+  | Node l _ r -> leaf_count l + leaf_count r
   | _ -> 1
 
 let max_leaf_count (t: tree): Tot pos = pow2 (height t)
 
 let rec bit_length (t: tree) (h: nat): Tot nat =
   match t with
-  | Node l r ->
+  | Node l _ r ->
     if h = 0 then 0 else bit_length l (h - 1) + bit_length r (h - 1)
   | _ ->
     if h = 0 then 1 else 0
@@ -49,6 +296,15 @@ val lemma_max_leaf_count: (t: tree) -> Lemma
 val lemma_non_full_bit_length: (t: tree) -> (h: nat) -> Lemma
   (requires leaf_count t < pow2 h)
   (ensures exists i. i < h /\ bit_length t i > 0)
+
+let rec lemma_leaf_count_height (t: tree): Lemma
+  (ensures height t < leaf_count t)
+  [SMTPat (height t)] =
+  match t with
+  | Node l _ r ->
+    lemma_leaf_count_height l;
+    lemma_leaf_count_height r
+  | _ -> ()
 
 let kraft_sum (len: seq pos): Tot rat =
   if length len = 0 then
